Tidying Theory

IRGraph.thy
@@ -1,16 +1,18 @@
-section \<open>GraalVM graph representation\<close>
+section \<open>GraalVM Graph Representation\<close>
 
 theory IRGraph
   imports 
     IRNodes
     "HOL-Library.FSet"
-    "HOL-Library.Finite_Map"
     "HOL.Relation"
 begin
 
-(* This theory defines the main Graal data structure - an entire IR Graph. 
-type_synonym RealGraph = "(ID fset \<times> (ID \<rightharpoonup> IRNode))" *)
+text \<open>This theory defines the main Graal data structure - an entire IR Graph.\<close>
 
+text \<open>
+IRGraph is defined as a partial map with a finite domain.
+The finite domain is required to be able to generate code and produce an interpreter.
+\<close>
 text_raw \<open>\Snip{graphdef}\<close>
 typedef IRGraph = "{g :: ID \<rightharpoonup> IRNode . finite (dom g)}"
 proof -
@@ -19,57 +21,30 @@ proof -
 qed
 text_raw \<open>\EndSnip\<close>
 
-(*
-fun is_valid :: "RealGraph \<Rightarrow> bool" where
-  "is_valid g = (\<forall> n . n |\<in>| fst g \<longleftrightarrow> n \<in> dom (snd g))"
-*)
-
-lemma valid_creation[simp]:
-  assumes "finite (dom g)"
-  shows "Rep_IRGraph (Abs_IRGraph g) = g"
-  using Abs_IRGraph_inverse assms by auto
-
-
-(*typedef IRGraph = "{g :: (ID fset \<times> (ID \<rightharpoonup> IRNode)) 
-                    . (\<forall> n . n |\<notin>| fst g \<longrightarrow> n \<notin> dom (snd g))}"*)
-
 setup_lifting type_definition_IRGraph
 
 lift_definition ids :: "IRGraph \<Rightarrow> ID set"
   is Map.dom .
 
+lift_definition kind :: "IRGraph \<Rightarrow> (ID \<rightharpoonup> IRNode)"
+  is Rep_IRGraph .
+
 lift_definition irgraph :: "(ID \<times> IRNode) list \<Rightarrow> IRGraph"
   is map_of
   by (simp add: finite_dom_map_of)
 
-lift_definition kind :: "IRGraph \<Rightarrow> (ID \<rightharpoonup> IRNode)"
-  is Rep_IRGraph .
+(* Theories are required for code generation to work *)
+code_datatype irgraph
 
 lemma irgraph[code]: "ids (irgraph m) = set (map fst m)"
   by transfer (simp add: dom_map_of_conv_image_fst ids.rep_eq irgraph.rep_eq)
 
-(* Get ALL the IDs in the graph. *)
-(*fun ids :: "IRGraph \<Rightarrow> ID set" where
-  "ids g = dom (Rep_IRGraph g)"*)
+lemma [code]: "(Rep_IRGraph (irgraph m)) = map_of m"
+  using Abs_IRGraph_inverse
+  by (simp add: irgraph.rep_eq)
+
 
 text_raw \<open>\Snip{helpers}%\<close>
-(* Look up a given ID in the graph and return the whole node. 
-definition kind :: "IRGraph \<Rightarrow> ID \<Rightarrow> IRNode option" where
-  "kind = snd"
-
-
-lemma simp_kind_def[simp]:
-  "kind g n = snd g n"
-  by (simp add: kind_def)
-lemma elim_kind_def[simp,elim]: 
-  assumes "x = kind g n"
-  shows "x = snd g n"
-  by (simp add: assms kind_def)
-*)
-
-lemma [simp]: "finite (ids g)"
-  using Rep_IRGraph ids.rep_eq by auto
-
 (* Get the inputs list of a given node ID. *)
 fun inp :: "IRGraph \<Rightarrow> ID \<Rightarrow> ID list" where
   "inp g nid = (case kind g nid of Some n \<Rightarrow> inputs_of n | None \<Rightarrow> [])"
@@ -82,10 +57,6 @@ fun input_edges :: "IRGraph \<Rightarrow> ID rel" where
 (* Find all the nodes in the graph that have nid as an input. *)
 fun usages :: "IRGraph \<Rightarrow> ID \<Rightarrow> ID set" where
   "usages g nid = {j. j \<in> ids g \<and> (j,nid) \<in> input_edges g}"
-text_raw \<open>\EndSnip\<close>
-(* usages WAS:
-  "usages g nid = fset (ffilter (\<lambda> nid' . nid \<in> set(inp g nid')) (fmdom g))"
-*)
 
 fun successor_edges :: "IRGraph \<Rightarrow> ID rel" where
   "successor_edges g = (\<Union> i \<in> ids g. {(i,j)|j . j \<in> fset(fset_of_list (succ  g i))})"
@@ -96,75 +67,6 @@ fun predecessors :: "IRGraph \<Rightarrow> ID \<Rightarrow> ID list" where
 fun is_empty :: "IRGraph \<Rightarrow> bool" where
   "is_empty g = ((ids g = {}) \<and> (kind g = Map.empty))"
 
-
-(* First well-formedness predicate for IR graphs.
-   This function uses field names.
-*
-fun wff_graph :: "IRGraph \<Rightarrow> bool" where
-  "wff_graph g = (
-    0 \<in> g_ids g \<and>
-    g_nodes g 0 = StartNode \<and>
-    (\<forall> n. n \<in> g_ids g \<longrightarrow> set(g_successors g n) \<subseteq> g_ids g) \<and>
-    (\<forall> n. n \<in> g_ids g \<longrightarrow> set(g_inputs g n) \<subseteq> g_ids g)
-  )
-  "
-*)
-(* Alternative definition using pattern matching.
-  TODO: add invariants about no loops through input arrows?
-       (certainly ShortCircuitOrNode.canonicalizeNegation assumes 
-
-   (and also through successor arrows?)
-*)
-
-(* We define these helper functions to make it easier to debug non-well-formed graphs.
-   E.g. if "wff_graph g" 
-   fails then try to prove each of:
-       "(\<forall>n. has_good_inputs n g)"
-       "(\<forall>n. has_good_successors n g)"
-       "(\<forall>n. wff_node (g_nodes g n) (g_inputs g n) (g_successors g n))"
-   and use 'nitpick' to find the bad n.
-*)
-
-(* graph closure invariants *)
-text_raw \<open>\Snip{graphinvar}%\<close>
-fun has_good_inputs :: "ID \<Rightarrow> IRGraph \<Rightarrow> bool" where
-  "has_good_inputs n g = list_all (\<lambda>i. i \<in> ids g) (inp g n)"
-
-fun has_good_successors :: "ID \<Rightarrow> IRGraph \<Rightarrow> bool" where
-  "has_good_successors n g = list_all (\<lambda>i. i \<in> ids g) (succ g n)"
-
-fun wff_graph :: "IRGraph \<Rightarrow> bool" where
-  "wff_graph g = (
-    0 \<in> ids g \<and> isType is_StartNode (kind g 0) \<and> 
-    (\<forall> n. n \<in> ids g \<longrightarrow> 
-      set (inp g n) \<subseteq> ids g \<and>
-      set (succ g n) \<subseteq> ids g \<and>
-      kind g n \<noteq> None))" (* \<and>
-    (\<not>(is_empty g) \<longrightarrow> 
-      (case kind g 0 of None \<Rightarrow> False | Some n \<Rightarrow> is_StartNode n)) \<and> 
-    (\<forall> n. n \<in> ids g \<longrightarrow> n \<in> dom (snd g))
-      has_good_inputs n g \<and>
-      has_good_successors n g \<and>
-   )"*)
-text_raw \<open>\EndSnip\<close>
-(* TODO: add these other invariants?
-    (\<forall> n. n \<notin> ids \<longrightarrow> nodes n = StartNode) \<and>
-    (\<forall> n. n \<notin> ids \<longrightarrow> successors n = []) \<and>
-    (\<forall> n. n \<notin> ids \<longrightarrow> inputs n = []) \<and>
-    (\<forall> n. n \<in> ids \<longrightarrow> wff_node (nodes n) (inputs n) (successors n))
-  )
-  "
-*)
-
-lemma wff_kind [simp]:
-  assumes "wff_graph g"
-  assumes "n \<in> ids g"
-  shows "kind g n \<noteq> None"
-  using wff_graph.simps  assms by auto
-
-(*fun irgraph :: "(ID \<times> IRNode) list \<Rightarrow> (ID \<rightharpoonup> IRNode)" where
-  "irgraph g = map_of g"*)
-
 fun add_node :: "nat \<Rightarrow> IRNode \<Rightarrow> IRGraph \<Rightarrow> IRGraph" where
   "add_node nid node g = 
     Abs_IRGraph ((kind g)(nid \<mapsto> node))"
@@ -172,18 +74,27 @@ fun add_node :: "nat \<Rightarrow> IRNode \<Rightarrow> IRGraph \<Rightarrow> IR
 fun remove_node :: "nat \<Rightarrow> IRGraph \<Rightarrow> IRGraph" where
   "remove_node nid g =
     Abs_IRGraph ((kind g)(nid := None))"
+text_raw \<open>\EndSnip\<close>
 
-(*
-lemma add_node_valid[simp]:         
-  assumes "gup = add_node nid k g"
-  shows "is_valid (Rep_IRGraph gup)"
-  using Rep_IRGraph by auto
 
-lemma remove_node_valid[simp]:
-  assumes "gup = remove_node nid g"
-  shows "is_valid (Rep_IRGraph gup)"
-  using Rep_IRGraph by auto
-*)
+text_raw \<open>\Snip{wff_graph}%\<close>
+fun wff_graph :: "IRGraph \<Rightarrow> bool" where
+  "wff_graph g = (
+    0 \<in> ids g \<and> isType is_StartNode (kind g 0) \<and> 
+    (\<forall> n. n \<in> ids g \<longrightarrow> 
+      set (inp g n) \<subseteq> ids g \<and>
+      set (succ g n) \<subseteq> ids g \<and>
+      kind g n \<noteq> None)
+  )"
+text_raw \<open>\EndSnip\<close>
+
+lemma ids_some[simp]: "x \<in> ids g \<longleftrightarrow> kind g x \<noteq> None" using ids.rep_eq kind_def by auto
+
+lemma valid_creation[simp]:
+  "finite (dom g) \<longleftrightarrow> Rep_IRGraph (Abs_IRGraph g) = g"
+  using Abs_IRGraph_inverse by (metis Rep_IRGraph mem_Collect_eq)
+
+lemma [simp]: "finite (ids g)" using Rep_IRGraph ids.rep_eq by auto
 
 lemma [simp]: "finite (ids (irgraph g))" by (simp add: finite_dom_map_of)
 
@@ -196,14 +107,15 @@ lemma [simp]: "ids (irgraph g) = set (map fst g)" using irgraph by auto
 lemma [simp]: "kind (irgraph g) = map_of g" using irgraph.rep_eq kind.transfer by auto
 
 
-(* Example 1: empty graph (just a start and end node) *)
+subsection "Example Graphs"
+text "Example 1: empty graph (just a start and end node)"
 definition start_end_graph:: IRGraph where
   "start_end_graph = irgraph [(0, StartNode None 1), (1, EndNode)]"
 
 lemma wff_empty: "wff_graph start_end_graph"
   unfolding start_end_graph_def wff_graph.simps by simp
 
-(* Example 2:
+text \<open>Example 2:
   public static int sq(int x) { return x * x; }
 
              [1 P(0)]
@@ -212,7 +124,7 @@ lemma wff_empty: "wff_graph start_end_graph"
        |      /
        V     /
       [5 Return]
-*)
+\<close>
 definition eg2_sq :: "IRGraph" where
   "eg2_sq = irgraph [
     (0, StartNode None 5),
@@ -221,35 +133,8 @@ definition eg2_sq :: "IRGraph" where
     (5, ReturnNode (Some 4) None)
    ]"
 
-lemma ids_some: "x \<in> ids g \<longleftrightarrow> kind g x \<noteq> None"
-  using ids.rep_eq kind_def by auto
-
-
-(* Now check some basic properties of this example. *)
 lemma wff_eg2_sq: "wff_graph eg2_sq"
   unfolding eg2_sq_def wff_graph.simps by simp
-  
-(*
-proof -
-  have wff_0: "0 \<in> ids eg2_sq"
-    unfolding eg2_sq_def eg2_sq_rep_def esy_ids by simp
-  have wff_1: "kind eg2_sq 0 = Some (StartNode None 5)" 
-    unfolding eg2_sq_def eg2_sq_rep_def esy_kind by simp
-  have wff_2: "\<forall> n \<in> ids eg2_sq . set (inp eg2_sq n) \<subseteq> ids eg2_sq"
-    unfolding eg2_sq_def eg2_sq_rep_def esy_ids esy_kind inp.simps by simp
-  have wff_3: "\<forall> n \<in> ids eg2_sq . set (succ eg2_sq n) \<subseteq> ids eg2_sq"
-    unfolding eg2_sq_def eg2_sq_rep_def esy_ids esy_kind succ.simps by simp
-  have wff_4: "\<forall> n \<in> ids eg2_sq . kind eg2_sq n \<noteq> None"
-    using ids_some by simp
-  from wff_0 wff_1 wff_2 wff_3 wff_4 show ?thesis unfolding wff_graph.simps by simp
-qed
-*)
-
-code_datatype Abs_IRGraph irgraph
-
-lemma [code]: "(Rep_IRGraph (irgraph m)) = map_of m"
-  using Abs_IRGraph_inverse
-  by (simp add: irgraph.rep_eq)
 
 (* Test the code generation. *)
 value "input_edges eg2_sq"
