ROOT
@@ -1,12 +1,13 @@
 session semantics = "HOL-Library" +
   description
     "GraalIR Semantics"
-  options [document = pdf, quick_and_dirty, show_question_marks = false]
+  options [document = pdf, document_output = "output", quick_and_dirty, show_question_marks = false]
   theories
     IRNodes
     IRGraph
     IREval
     IRStepObj
-    Canonicalization
+    (*Canonicalization*)
   document_files
     "root.tex"
+    "mathpartir.sty"
